spec/Correctness.ec
@@ -2,13 +2,13 @@ pragma Goals : printall.
 
 (**********************************************************************************************************************)
 
-require import Address Notation Parameters Primitives Properties Wots.
-
 (* proof that the extracted EasyCrypt is equiavalent to the (preprocessed)1 EasyCrypt *)
 (* The preprocessed EasyCrypt is the same as the extracted EasyCrypt, but replaces calls to core_hash with calls
    to an operator H *)
 
 require import XMSS_IMPL.
 require import XMSS_IMPL_PP.
+
+require import Address.
 
 
