spec/extraction/XMSS_IMPL.ec
@@ -877,19 +877,19 @@ module M(SC:Syscall_t) = {
     return (out);
   }
   
-  proc __core_hash_96 (out:W8.t Array32.t, in_0:W8.t Array96.t) : W8.t Array32.t = {
-    
-    
-    
-    out <@ __sha256_96 (out, in_0);
-    return (out);
-  }
-  
   proc __core_hash_128 (out:W8.t Array32.t, in_0:W8.t Array128.t) : W8.t Array32.t = {
     
     
     
     out <@ __sha256_128 (out, in_0);
+    return (out);
+  }
+  
+  proc __core_hash_96 (out:W8.t Array32.t, in_0:W8.t Array96.t) : W8.t Array32.t = {
+    
+    
+    
+    out <@ __sha256_96 (out, in_0);
     return (out);
   }
   
@@ -1149,6 +1149,66 @@ module M(SC:Syscall_t) = {
     return ();
   }
   
+  proc __memcpy_u8u8_64_64 (out:W8.t Array64.t, offset:W64.t,
+                            in_0:W8.t Array64.t) : W8.t Array64.t * W64.t = {
+    
+    var i:W64.t;
+    
+    i <- (W64.of_int 0);
+    
+    while ((i \ult (W64.of_int 64))) {
+      out.[(W64.to_uint offset)] <- in_0.[(W64.to_uint i)];
+      i <- (i + (W64.of_int 1));
+      offset <- (offset + (W64.of_int 1));
+    }
+    return (out, offset);
+  }
+  
+  proc __memcpy_u8u8_128_64 (out:W8.t Array128.t, offset:W64.t,
+                             in_0:W8.t Array64.t) : W8.t Array128.t * W64.t = {
+    
+    var i:W64.t;
+    
+    i <- (W64.of_int 0);
+    
+    while ((i \ult (W64.of_int 64))) {
+      out.[(W64.to_uint offset)] <- in_0.[(W64.to_uint i)];
+      i <- (i + (W64.of_int 1));
+      offset <- (offset + (W64.of_int 1));
+    }
+    return (out, offset);
+  }
+  
+  proc __memcpy_u8u8_64_32 (out:W8.t Array64.t, offset:W64.t,
+                            in_0:W8.t Array32.t) : W8.t Array64.t * W64.t = {
+    
+    var i:W64.t;
+    
+    i <- (W64.of_int 0);
+    
+    while ((i \ult (W64.of_int 32))) {
+      out.[(W64.to_uint offset)] <- in_0.[(W64.to_uint i)];
+      i <- (i + (W64.of_int 1));
+      offset <- (offset + (W64.of_int 1));
+    }
+    return (out, offset);
+  }
+  
+  proc __memcpy_u8u8_128_32 (out:W8.t Array128.t, offset:W64.t,
+                             in_0:W8.t Array32.t) : W8.t Array128.t * W64.t = {
+    
+    var i:W64.t;
+    
+    i <- (W64.of_int 0);
+    
+    while ((i \ult (W64.of_int 32))) {
+      out.[(W64.to_uint offset)] <- in_0.[(W64.to_uint i)];
+      i <- (i + (W64.of_int 1));
+      offset <- (offset + (W64.of_int 1));
+    }
+    return (out, offset);
+  }
+  
   proc __memcpy_u8u8_96_32 (out:W8.t Array96.t, offset:W64.t,
                             in_0:W8.t Array32.t) : W8.t Array96.t * W64.t = {
     
@@ -1179,66 +1239,6 @@ module M(SC:Syscall_t) = {
     return (out, offset);
   }
   
-  proc __memcpy_u8u8_128_64 (out:W8.t Array128.t, offset:W64.t,
-                             in_0:W8.t Array64.t) : W8.t Array128.t * W64.t = {
-    
-    var i:W64.t;
-    
-    i <- (W64.of_int 0);
-    
-    while ((i \ult (W64.of_int 64))) {
-      out.[(W64.to_uint offset)] <- in_0.[(W64.to_uint i)];
-      i <- (i + (W64.of_int 1));
-      offset <- (offset + (W64.of_int 1));
-    }
-    return (out, offset);
-  }
-  
-  proc __memcpy_u8u8_64_64 (out:W8.t Array64.t, offset:W64.t,
-                            in_0:W8.t Array64.t) : W8.t Array64.t * W64.t = {
-    
-    var i:W64.t;
-    
-    i <- (W64.of_int 0);
-    
-    while ((i \ult (W64.of_int 64))) {
-      out.[(W64.to_uint offset)] <- in_0.[(W64.to_uint i)];
-      i <- (i + (W64.of_int 1));
-      offset <- (offset + (W64.of_int 1));
-    }
-    return (out, offset);
-  }
-  
-  proc __memcpy_u8u8_128_32 (out:W8.t Array128.t, offset:W64.t,
-                             in_0:W8.t Array32.t) : W8.t Array128.t * W64.t = {
-    
-    var i:W64.t;
-    
-    i <- (W64.of_int 0);
-    
-    while ((i \ult (W64.of_int 32))) {
-      out.[(W64.to_uint offset)] <- in_0.[(W64.to_uint i)];
-      i <- (i + (W64.of_int 1));
-      offset <- (offset + (W64.of_int 1));
-    }
-    return (out, offset);
-  }
-  
-  proc __memcpy_u8u8_64_32 (out:W8.t Array64.t, offset:W64.t,
-                            in_0:W8.t Array32.t) : W8.t Array64.t * W64.t = {
-    
-    var i:W64.t;
-    
-    i <- (W64.of_int 0);
-    
-    while ((i \ult (W64.of_int 32))) {
-      out.[(W64.to_uint offset)] <- in_0.[(W64.to_uint i)];
-      i <- (i + (W64.of_int 1));
-      offset <- (offset + (W64.of_int 1));
-    }
-    return (out, offset);
-  }
-  
   proc __memcpy_u8u8_2144_32 (out:W8.t Array2144.t, offset:W64.t,
                               in_0:W8.t Array32.t) : W8.t Array2144.t * W64.t = {
     
@@ -1251,6 +1251,42 @@ module M(SC:Syscall_t) = {
       i <- (i + (W64.of_int 1));
       offset <- (offset + (W64.of_int 1));
     }
+    return (out, offset);
+  }
+  
+  proc _memcpy_u8u8_64_64 (out:W8.t Array64.t, offset:W64.t,
+                           in_0:W8.t Array64.t) : W8.t Array64.t * W64.t = {
+    
+    
+    
+    (out, offset) <@ __memcpy_u8u8_64_64 (out, offset, in_0);
+    return (out, offset);
+  }
+  
+  proc _memcpy_u8u8_128_64 (out:W8.t Array128.t, offset:W64.t,
+                            in_0:W8.t Array64.t) : W8.t Array128.t * W64.t = {
+    
+    
+    
+    (out, offset) <@ __memcpy_u8u8_128_64 (out, offset, in_0);
+    return (out, offset);
+  }
+  
+  proc _memcpy_u8u8_64_32 (out:W8.t Array64.t, offset:W64.t,
+                           in_0:W8.t Array32.t) : W8.t Array64.t * W64.t = {
+    
+    
+    
+    (out, offset) <@ __memcpy_u8u8_64_32 (out, offset, in_0);
+    return (out, offset);
+  }
+  
+  proc _memcpy_u8u8_128_32 (out:W8.t Array128.t, offset:W64.t,
+                            in_0:W8.t Array32.t) : W8.t Array128.t * W64.t = {
+    
+    
+    
+    (out, offset) <@ __memcpy_u8u8_128_32 (out, offset, in_0);
     return (out, offset);
   }
   
@@ -1272,39 +1308,59 @@ module M(SC:Syscall_t) = {
     return (out, offset);
   }
   
-  proc _memcpy_u8u8_128_64 (out:W8.t Array128.t, offset:W64.t,
-                            in_0:W8.t Array64.t) : W8.t Array128.t * W64.t = {
+  proc _x_memcpy_u8u8_64_64 (out:W8.t Array64.t, offset:W64.t,
+                             in_0:W8.t Array64.t) : W8.t Array64.t * W64.t = {
     
     
     
-    (out, offset) <@ __memcpy_u8u8_128_64 (out, offset, in_0);
+    out <- out;
+    offset <- offset;
+    in_0 <- in_0;
+    (out, offset) <@ _memcpy_u8u8_64_64 (out, offset, in_0);
+    out <- out;
+    offset <- offset;
     return (out, offset);
   }
   
-  proc _memcpy_u8u8_64_64 (out:W8.t Array64.t, offset:W64.t,
-                           in_0:W8.t Array64.t) : W8.t Array64.t * W64.t = {
+  proc _x_memcpy_u8u8_128_64 (out:W8.t Array128.t, offset:W64.t,
+                              in_0:W8.t Array64.t) : W8.t Array128.t * W64.t = {
     
     
     
-    (out, offset) <@ __memcpy_u8u8_64_64 (out, offset, in_0);
+    out <- out;
+    offset <- offset;
+    in_0 <- in_0;
+    (out, offset) <@ _memcpy_u8u8_128_64 (out, offset, in_0);
+    out <- out;
+    offset <- offset;
     return (out, offset);
   }
   
-  proc _memcpy_u8u8_128_32 (out:W8.t Array128.t, offset:W64.t,
-                            in_0:W8.t Array32.t) : W8.t Array128.t * W64.t = {
+  proc _x_memcpy_u8u8_64_32 (out:W8.t Array64.t, offset:W64.t,
+                             in_0:W8.t Array32.t) : W8.t Array64.t * W64.t = {
     
     
     
-    (out, offset) <@ __memcpy_u8u8_128_32 (out, offset, in_0);
+    out <- out;
+    offset <- offset;
+    in_0 <- in_0;
+    (out, offset) <@ _memcpy_u8u8_64_32 (out, offset, in_0);
+    out <- out;
+    offset <- offset;
     return (out, offset);
   }
   
-  proc _memcpy_u8u8_64_32 (out:W8.t Array64.t, offset:W64.t,
-                           in_0:W8.t Array32.t) : W8.t Array64.t * W64.t = {
+  proc _x_memcpy_u8u8_128_32 (out:W8.t Array128.t, offset:W64.t,
+                              in_0:W8.t Array32.t) : W8.t Array128.t * W64.t = {
     
     
     
-    (out, offset) <@ __memcpy_u8u8_64_32 (out, offset, in_0);
+    out <- out;
+    offset <- offset;
+    in_0 <- in_0;
+    (out, offset) <@ _memcpy_u8u8_128_32 (out, offset, in_0);
+    out <- out;
+    offset <- offset;
     return (out, offset);
   }
   
@@ -1331,62 +1387,6 @@ module M(SC:Syscall_t) = {
     offset <- offset;
     in_0 <- in_0;
     (out, offset) <@ _memcpy_u8u8_32_32 (out, offset, in_0);
-    out <- out;
-    offset <- offset;
-    return (out, offset);
-  }
-  
-  proc _x_memcpy_u8u8_128_64 (out:W8.t Array128.t, offset:W64.t,
-                              in_0:W8.t Array64.t) : W8.t Array128.t * W64.t = {
-    
-    
-    
-    out <- out;
-    offset <- offset;
-    in_0 <- in_0;
-    (out, offset) <@ _memcpy_u8u8_128_64 (out, offset, in_0);
-    out <- out;
-    offset <- offset;
-    return (out, offset);
-  }
-  
-  proc _x_memcpy_u8u8_64_64 (out:W8.t Array64.t, offset:W64.t,
-                             in_0:W8.t Array64.t) : W8.t Array64.t * W64.t = {
-    
-    
-    
-    out <- out;
-    offset <- offset;
-    in_0 <- in_0;
-    (out, offset) <@ _memcpy_u8u8_64_64 (out, offset, in_0);
-    out <- out;
-    offset <- offset;
-    return (out, offset);
-  }
-  
-  proc _x_memcpy_u8u8_128_32 (out:W8.t Array128.t, offset:W64.t,
-                              in_0:W8.t Array32.t) : W8.t Array128.t * W64.t = {
-    
-    
-    
-    out <- out;
-    offset <- offset;
-    in_0 <- in_0;
-    (out, offset) <@ _memcpy_u8u8_128_32 (out, offset, in_0);
-    out <- out;
-    offset <- offset;
-    return (out, offset);
-  }
-  
-  proc _x_memcpy_u8u8_64_32 (out:W8.t Array64.t, offset:W64.t,
-                             in_0:W8.t Array32.t) : W8.t Array64.t * W64.t = {
-    
-    
-    
-    out <- out;
-    offset <- offset;
-    in_0 <- in_0;
-    (out, offset) <@ _memcpy_u8u8_64_32 (out, offset, in_0);
     out <- out;
     offset <- offset;
     return (out, offset);
